\subsection{Introduction}

\subsubsection{Quadratic Equations}
 
{\tmstrong{After simplifying, classify each equation as linear, quadratic, or neither.
 If the equation is a quadratic, then specify whether it is concave up or down.}}

\begin{multicols}{2}
  1)~$y=x^2 + 9$\\
	3)~$y=x+6-3x$\\
	5)~$y=-5x+3+2x-3x^2+6$\\
  7)~$y=(x-1)(x+2)+3$\\
  9)~$y=(x-4)(x+4)-(x+1)^2$\\
	2)~$y=5-2x+x^2$\\
	4)~$y=5x+x^2-3x-3x^2$\\
  6)~$y=3x^2+-x+x-3x^2+6$\\
  8)~$y=(x-5)(2x+3)-2(x-3)$\\
  10)~$y=(2x-4)(x-1)-2(x+3)^2+3x^2$
\end{multicols}

~\\%\newpage

\subsubsection{An Introduction to the Vertex Form} 

{\tmstrong{Identify the vertex and concavity (concave up or down) of each quadratic.}}

\begin{multicols}{2}
  1)~$y=(x-3)^2+4$\\
  3)~$y=6(x+3)^2+4$\\
  5)~$y=-2(x-1)^2-7$\\
  7)~$y=7x^2+4$\\
  9)~$y=x^2+4$\\
  2)~$y=(x-2)^2+5$\\
  4)~$y=-2(x-3)^2+4$\\
  6)~$y=-(x+1)^2$\\
  8)~$y=-\frac{1}{23}(x-8)^2+5$\\
  10)~$y=5x^2+23$
\end{multicols}

\newpage

\subsection{Factoring}

\subsubsection{Greatest Common Factor}

{\tmstrong{Factor the common factor out of each expression.}}

\begin{multicols}{2}
  1)~ $4 + 8 b^2$\\
  3)~ $45 x^2 - 25$\\
  5)~ $56 - 35 p$\\
  7)~ $7 ab - 35 a^2 b$\\
  9)~ $- 3 a^2 b + 6 a^3 b^2$\\
  11)~ $- 5 x^2 - 5 x^3 - 15 x^4$\\
  13)~ $20 x^4 - 30 x + 30$\\
  15)~ $28 m^4 + 40 m^3 + 8$\\
  17)~ $30 b^9 + 5 a b - 15 a^2$\\
  19)~ $- 48 a^2 b^2 - 56 a^3 b - 56 a^5 b$\\
  21)~ $20 x^8 y^2 z^2 + 15 x^5 y^2 z + 35 x^3 y^3 z$\\
  23)~ $50 x^2 y + 10 y^2 + 70 x z^2$\\
  25)~ $30 q p r - 5 q p + 5 q$\\
  27)~ $- 18 n^5 + 3 n^3 - 21 n + 3$\\
  29)~ $- 40 x^{11} - 20 x^{12} + 50 x^{13} - 50 x^{14}$\\
  31)~ $- 32 m n^8 + 4 m^6 n + 12 m n^4 + 16 m n$\\
~\\
  2)~ $x - 5$\\
  4)~ $-n - 2 n^2$\\
  6)~ $50 x - 80 y$\\
  8)~ $27 x^2 y^5 - 72 x^3 y^2$\\
  10)~ $8 x^3 y^2 + 4 x^3$\\
  12)~ $- 32 n^9 + 32 n^6 + 40 n^5$\\
  14)~ $21 p^6 + 30 p^2 + 27$\\
  16)~ $- 10 x^4 + 20 x^2 + 12 x$\\
  18)~ $27 y^7 + 12 y^2 x + 9 y^2$\\
  20)~ $30 m^6 + 15 m n^2 - 25$\\
  22)~ $3 p + 12 q - 15 q^2 r^2$\\
  24)~ $30 y^4 z^3 x^5 + 50 y^4 z^5 - 10 y^4 z^3 x$\\
  26)~ $28 b + 14 b^2 + 35 b^3 + 7 b^5$\\
  28)~ $30 a^8 + 6 a^5 + 27 a^3 + 21 a^2$\\
  30)~ $- 24 x^6 - 4 x^4 + 12 x^3 + 4 x^2$\\
  32)~ $- 10 y^7 + 6 y^{10} - 4 y^{10} x - 8 y^8 x$
\end{multicols}

%\newpage

\subsubsection{Grouping}

{\tmstrong{Factor each expression completely.}}

\begin{multicols}{2}
  1)~ $40 r^3 - 8 r^2 - 25 r + 5$\\
  3)~ $3 n^3 - 2 n^2 - 9 n + 6$\\
  5)~ $15 b^3 + 21 b^2 - 35 b - 49$\\
  7)~ $3 x^3 + 15 x^2 + 2 x + 10$\\
  9)~ $35 x^3 - 28 x^2 - 20 x + 16$\\
  11)~ $7 x y - 49 x + 5 y - 35$\\
  13)~ $32 x y + 40 x^2 + 12 y + 15 x$\\
  15)~ $16 x y - 56 x + 2 y - 7$\\
  17)~ $2 x y - 8 x^2 + 7 y^3 - 28 y^2 x$\\
  19)~ $40 x y + 35 x - 8 y^2 - 7 y$\\
  21)~ $32 u v - 20 u + 24 v - 15$\\
  23)~ $10 x y + 30 + 25 x + 12 y$\\
  25)~ $3 u v + 14 u - 6 u^2 - 7 v$\\
  27)~ $16 x y - 3 x - 6 x^2 + 8 y$\\
  2)~ $35 x^3 - 10 x^2 - 56 x + 16$\\
  4)~ $14 v^3 + 10 v^2 - 7 v - 5$\\
  6)~ $6 x^3 - 48 x^2 + 5 x - 40$\\
  8)~ $28 p^3 + 21 p^2 + 20 p + 15$\\
  10)~ $7 n^3 + 21 n^2 - 5 n - 15$\\
  12)~ $42 r^3 - 49 r^2 + 18 r - 21$\\
  14)~ $15 a b - 6 a + 5 b^3 - 2 b^2$\\
  16)~ $3 m n - 8 m + 15 n - 40$\\
  18)~ $5 m n + 2 m - 25 n - 10$\\
  20)~ $8 x y + 56 x - y - 7$\\
  22)~ $4 u v + 14 u^2 + 12 v + 42 u$\\
  24)~ $24 x y + 25 y^2 - 20 x - 30 y^3$\\
  26)~ $56 a b + 14 - 49 a - 16 b$
\end{multicols}

\newpage

\subsubsection{Trinomials with Leading Coefficient $a=1$}

{\tmstrong{Factor each expression completely.}}
\label{ais1}
\begin{multicols}{2}
  1)~ $p^2 + 17 p + 72$\\
  3)~ $n^2 - 9 n + 8$\\
  5)~ $x^2 - 9 x - 10$\\
  7)~ $b^2 + 12 b + 32$\\
  9)~ $x^2 + 3 x - 70$\\
  11)~ $n^2 - 8 n + 15$\\
  13)~ $p^2 + 15 p + 54$\\
  15)~ $n^2 - 15 n + 56$\\
  17)~ $u^2 - 8 u v + 15 v^2$\\
  19)~ $m^2 + 2 m n - 8 n^2$\\
  21)~ $x^2 - 11 x y + 18 y^2$\\
  23)~ $x^2 + x y - 12 y^2$\\
  25)~ $x^2 + 4 x y - 12 y^2$\\
  27)~ $5 a^2 + 60 a + 100$\\
  29)~ $6 a^2 + 24 a - 192$\\
  31)~ $6 x^2_{} + 18 x y + 12 y^2$\\
  33)~ $6 x^2 + 96 x y + 378 y^2$\\
~\\
  2)~ $x^2_{} + x - 72$\\
  4)~ $x^2 + x - 30$\\
  6)~ $x^2 + 13 x + 40$\\
  8)~ $b^2 - 17 b + 70$\\
  10)~ $x^2 + 3 x - 18$\\
  12)~ $a^2 - 6 a - 27$\\
  14)~ $p^2 + 7 p - 30$\\
  16)~ $m^2 - 15 m n + 50 n^2$\\
  18)~ $m^2 - 3 m n - 40 n^2$\\
  20)~ $x^2 + 10 x y + 16 y^2$\\
  22)~ $u^2 - 9 u v + 14 v^2$\\
  24)~ $x^2 + 14 x y + 45 y^2$\\
  26)~ $4 x^2 + 52 x + 168$\\
  28)~ $5 n^2 - 45 n + 40$\\
  30)~ $5 v^2 + 20 v - 25$\\
  32)~ $5 m^2 + 30 m n - 90 n^2$\\
  34)~ $6 m^2 - 36 m n - 162 n^2$
\end{multicols}

\newpage

\subsubsection{Trinomials with Leading Coefficient $a\neq 1$}

{\tmstrong{Factor each expression completely.}}
\label{aisnot1}
\begin{multicols}{2}
  1)~ $7 x^2 - 48 x + 36$\\
  3)~ $7 b^2 + 15 b + 2$\\
  5)~ $5 a^2 - 13 a - 28$\\
  7)~ $2 x^2 - 5 x + 2$\\
  9)~ $2 x^2 + 19 x + 35$\\
  11)~ $2 b^2 - b - 3$\\
  13)~ $5 x^2 + 13 x + 6$\\
  15)~ $3 x^2 - 17 x + 20$\\
  17)~ $3 x^2 + 17 x y + 10 y^2$\\
  19)~ $5 x^2 + 28 x y - 49 y^2$\\
  21)~ $6 x^2 - 39 x - 21$\\
  23)~ $21 x^2 - 87 x - 90$\\
  25)~ $14 x^2 - 60 x + 16$\\
  27)~ $6 x^2 + 29 x + 20$\\
  29)~ $4 x^2 - 17 x + 4$\\
  31)~ $4 x^2 + 9 x y + 2 y^2$\\
  33)~ $4 m^2 - 9 m n - 9 n^2$\\
  35)~ $4 x^2 + 13 x y + 3 y^2$\\
  37)~ $12 x^2 + 62 x y + 70 y^2$\\
  39)~ $24 x^2 - 52 x y + 8 y^2$\\
~\\
  2)~ $7 n^2 - 44 n + 12$\\
  4)~ $7 v^2 - 24 v - 16$\\
  6)~ $5 n^2 - 7 n - 24$\\
  8)~ $3 r^2 - 4 r - 4$\\
  10)~ $7 x^2 + 29 x - 30$\\
  12)~ $5 x^2 - 26 x + 24$\\
  14)~ $3 r^2 + 16 r + 21$\\
  16)~ $3 u^2 + 13 u v - 10 v^2$\\
  18)~ $7 x^2 - 2 x y - 5 y^2$\\
  20)~ $5 u^2 + 31 u v - 28 v^2$\\
  22)~ $10 a^2 - 54 a - 36$\\
  24)~ $21 n^2 + 45 n - 54$\\
  26)~ $4 r^2 + r - 3$\\
  28)~ $6 p^2 + 11 p - 7$\\
  30)~ $4 r^2 + 3 r - 7$\\
  32)~ $4 m^2 + 6 m n + 6 n^2$\\
  34)~ $4 x^2 - 6 x y + 30 y^2$\\
  36)~ $18 u^2 - 3 u v - 36 v^2$\\
  38)~ $16 x^2 + 60 x y + 36 y^2$\\
  40)~ $12 x^2 + 50 x y + 28 y^2$\\
\end{multicols}

\newpage

\subsection{Solving by Factoring}

{\tmstrong{Set each of the following expressions equal to zero and solve for the given variable.}}\pp

1) - 15): Expressions (1) through (15) on page \pageref{ais1}.\pp

16) - 30): Expressions (1) through (15) on page \pageref{aisnot1}.\pp

31) - 40): Expressions (21) through (30) on page \pageref{aisnot1}.

\newpage

\subsection{Vertex Form and Graphing}

\subsubsection{The Vertex Form}

{\tmstrong{Identify whether the quadratic is in vertex form, standard form, or both.  If it is in vertex form, then identify the vertex ($h,k$).}}

\begin{multicols}{2}
  1)~$y=(x-12)^2+5 $\\
  3)~$y=x^2+8$\\
  5)~$y=-4(x-1)^2+2$\\
  7)~$y=x^2+3x+4$\\
  9)~$y=x^2-3$\\
  11)~$y=(x-1)^2$\\
  2)~$y=-3(x-3)^2+5 $\\
  4)~$y=2(x-4)^2 $\\
  6)~$y=-5(x-7)^2$\\
  8)~$y=x^2-1$\\
  10)~$y=(x-1)^2-3 $\\
  12)~$y=x^2$
\end{multicols}

%~\vspace{1in}

{\tmstrong{Each quadratic equation below has been given in standard form.  Rewrite each equation in vertex form.}}

\begin{multicols}{2}
  13)~$y=x^2+2x-1 $\\
  15)~$y=3x^2+12x-1$\\
  17)~$y=x^2+6$\\
  19)~$y=x^2+8x$\\
  21)~$y=x^2+4x-2$\\
  23)~$y=4x^2+10x$\\
  14)~$y=-3x^2-12x-5 $\\
  16)~$y=x^2+2x$\\
  18)~$y=-5x^2-40x$\\
  20)~$y=x^2$\\
  22)~$y=x^2+16x-2 $
\end{multicols}

\subsubsection{Graphing Quadratics}

{\tmstrong{Find the vertex and intercepts of the following quadratics. Use
this information to graph the resulting parabola.}}

\begin{multicols}{2}
  1)~ $y = x^2 - 2 x - 8$\\
  3)~ $y = 2 x^2 - 12 x + 10$\\
  5)~ $y = - 2 x^2 + 12 x - 18$\\
  7)~ $y = - 3 x^2 + 24 x - 45$\\
  9)~ $y = - x^2 + 4 x_{} + 5$\\
  11)~ $y = - x^2 + 6 x - 5$\\
  13)~ $y = - 2 x^2 + 16 x - 24$\\
  15)~ $y = 3 x^2 + 12 x + 9$\\
  17)~ $y = 5 x^2 - 40 x + 75$\\
  19)~ $y = - 5 x^2 - 60 x - 175$\\
~\\
  2)~ $y = x^2 - 2 x - 3$\\
  4)~ $y = 2 x^2 - 12 x + 16$\\
  6)~ $y = - 2 x^2 + 12 x - 10$\\
  8)~ $y = - 3 x^2 + 12 x - 9$\\
  10)~ $y = - x^2 + 4 x - 3$\\
  12)~ $y = - 2 x^2 + 16 x - 30$\\
  14)~ $y = 2 x^2 + 4 x - 6$\\
  16)~ $y = 5 x^2 + 30 x + 45$\\
  18)~ $y = 5 x^2 + 20 x + 15$\\
  20)~ $y = - 5 x^2 + 20 x - 15$\\
\end{multicols}

\newpage

\subsection{Square Roots and the Imaginary Number $i$}

\subsubsection{Square Roots}

{\tmstrong{Simplify each of the following square roots completely.}}%\pp

\begin{multicols}{2}
	1)~ $\sqrt[]{245}$\\
  3)~ $\sqrt[]{36}$\\
  5)~ $\sqrt[]{12}$\\
  7)~ $3~\sqrt[]{12}$\\
  9)~ $6~\sqrt[]{128}$\\
  11)~ $- 8~\sqrt[]{392}$\\
  13)~ $\sqrt[]{192 n}$\\
  15)~ $\sqrt[]{196 v^2}$\\
  17)~ $\sqrt[]{252 x^2}$\\
  19)~ $-~\sqrt[]{100 k^4}$\\
  21)~ $- 7~\sqrt[]{64 x^4}$\\
  23)~ $- 5~\sqrt[]{36 m}$\\
  25)~ $\sqrt[]{45 x^2 y^2}$\\
  27)~ $\sqrt[]{16 x^3 y^3}$\\
  29)~ $\sqrt[]{320 x^4 y^4}$\\
  31)~ $6~\sqrt[]{80 x^{} y^2}$\\
  33)~ $5~\sqrt[]{245 x^2 y^3}$\\
  35)~ $- 2~\sqrt[]{180 u^3 v}$\\
  37)~ $- 8~\sqrt[]{180 x^4 y^2 z^4}$\\
  39)~ $2~\sqrt[]{80 h j^4 k}$\\
  41)~ $- 4~\sqrt[]{54 m n p^2}$\\
  ~\\
	2)~ $\sqrt[]{125}$\\
  4)~ $\sqrt[]{196}$\\
  6)~ $\sqrt[]{72}$\\
  8)~ $5~\sqrt[]{32}$\\
  10)~ $7~\sqrt[]{128}$\\
  12)~ $- 7~\sqrt[]{63}$\\
  14)~ $\sqrt[]{343 b}$\\
  16)~ $\sqrt[]{100 n^3}$\\
  18)~ $\sqrt[]{200 a^3}$\\
  20)~ $- 4~\sqrt[]{175 p^4}$\\
  22)~ $- 2~\sqrt[]{128 n}$\\
  24)~ $8~\sqrt[]{112 p^2}$\\
  26)~ $\sqrt[]{72 a^3 b^4}$\\
  28)~ $\sqrt[]{512 a^4 b^2}$\\
  30)~ $\sqrt[]{512 m^4 n^3}$\\
  32)~ $8~\sqrt[]{98 m n}$\\
  34)~ $2~\sqrt[]{72 x^2 y^2}$\\
  36)~ $- 5~\sqrt[]{72 x^3 y^4}$\\
  38)~ $6~\sqrt[]{50 a^4 b c^2}$\\
  40)~ $-~\sqrt[]{32 x y^2 z^3}$\\
  42)~ $- 8~\sqrt[]{32 m^2 p^4 q}$\\
\end{multicols}

\newpage

\subsubsection{Intro to Complex Numbers}

{\tmstrong{Rewrite each of the following complex numbers in the form $a+bi$, where $a$ and $b$ are real numbers and $i=\sqrt{-1}$.}}%\pp

\begin{multicols}{2}
  1)~ $3 - (- 8 + 4 i)$\\
  3)~ $(7 i) - (3 - 2 i)$\\
  5)~ $(- 6 i) - (3 + 7 i)$\\
  7)~ $(3 - 3 i) + (- 7 - 8 i)$\\
  9)~ $(i) - (2 + 3 i) - 6$\\
  11)~ $(6 i) (- 8 i)$\\
  13)~ $(- 5 i) (8 i)$\\
  15)~ $(- 7 i)^2$\\
  17)~ $(6 + 5 i)^2$\\
  19)~ $(- 7 - 4 i) (- 8 + 6 i)$\\
  21)~ $(- 4 + 5 i) (2 - 7 i)$\\
  23)~ $(- 8 - 6 i) (- 4 + 2 i)$\\
  25)~ $(1 + 5 i) (2 + i)$\\
  27)~ $\dfrac{- 9 + 5 i}{i}$\\
  29)~ $\dfrac{- 10 - 9 i}{6 i}$\\
  31)~ $\dfrac{- 3 - 6 i}{4 i}$\\
  33)~ $\dfrac{10 - i}{- i}$\\
  35)~ $\dfrac{4 i}{- 10 + i}$\\
  37)~ $\dfrac{8}{7 - 6 i}$\\
  39)~ $\dfrac{7}{10 - 7 i}$\\
  41)~ $\dfrac{5 i}{- 6 - i}$\\
  43)~ $\sqrt{- 81}$\\
  45)~ $\sqrt{- 10} \sqrt{- 2}$\\
  47~ $\frac{3 + \sqrt{- 27}}{6}$\\
  49)~ $\frac{8 - \sqrt{- 16}}{4}$\\
  51)~ $i^{73}$\\
  53)~ $i^{48}$\\
  55)~ $i^{62}$\\
  57)~ $i^{154}$\\
  2)~ $(3 i) - (7 i)$\\
  4)~ $5 + (- 6 - 6 i)$\\
  6)~ $(- 8 i) - (7 i) - (5 - 3 i)$\\
  8)~ $(- 4 - i) + (1 - 5 i)$\\
  10)~ $(5 - 4 i) + (8 - 4 i)$\\
  12)~ $(3 i) (- 8 i)$\\
  14)~ $(8 i) (- 4 i)$\\
  16)~ $(- i) (7 i) (4 - 3 i)$\\
  18)~ $(8 i) (- 2 i) (- 2 - 8 i)$\\
  20)~ $(3 i) (- 3 i) (4 - 4 i)$\\
  22)~ $- 8 (4 - 8 i) - 2 (- 2 - 6 i)$\\
  24)~ $(- 6 i) (3 - 2 i) - (7 i) (4 i)$\\
  26)~ $(- 2 + i) (3 - 5 i)$\\
  28)~ $\dfrac{- 3 + 2 i}{- 3 i}$\\
  30)~ $\dfrac{- 4 + 2 i}{3 i}$\\
  32)~ $\dfrac{- 5 + 9 i}{9 i}$\\
  34)~ $\dfrac{10}{5 i}$\\
  36)~ $\dfrac{9 i}{1 - 5 i}$\\
  38)~ $\dfrac{4}{4 + 6 i}$\\
  40)~ $\dfrac{9}{- 8 - 6 i}$\\
  42)~ $\dfrac{8 i}{6 - 7 i}$\\
%\end{multicols}
%\begin{multicols}{2}
  44)~ $\sqrt{- 45}$\\
  46)~ $\sqrt{- 12} \sqrt{- 2}$\\
  48)~ $\frac{- 4 - \sqrt{- 8}}{- 4}$\\
  50)~ $\frac{6 + \sqrt{- 32}}{4}$\\
  52)~ $i^{251}$\\
  54)~ $i^{68}$\\
  56)~ $i^{181}$\\
  58)~ $i^{51}$
\end{multicols}

\newpage

\subsection{Solving by Extracting Square Roots}

{\tmstrong{Find the $x$-intercepts of each quadratic by setting $y=0$ and using the method of extracting square roots.}}

\begin{multicols}{2}
  1)~$y=(x-12)^2-5 $\\
  3)~$y=x^2-16$\\
  5)~$y=-4(x-1)^2+20$\\
  7)~$y=-4(x+6)^2+8$\\
  9)~$y=(x-4)^2-9$\\
  11)$y=(x+2)^2+16$\\
  2)~$y=-3(x-3)^2+30 $\\
  4)~$y=2(x-4)^2 -200 $\\
  6)~$y=-2(x-7)^2+50$\\
  8)~$y=x^2-4$\\
  10)$y=(x-1)^2-25 $\\
  12)$y=9(x-11)^2-81$
\end{multicols}

\newpage

\subsection{Completing the Square}

{\tmstrong{Find the value that completes the square and then rewrite the given expression as a
perfect square.}}

\begin{multicols}{2}
  1)~ $x^2 - 30 x +$~\underline{\hspace{.5in}}\\
  3)~ $m^2 - 36 m +$~\underline{\hspace{.5in}}\\
  5)~ $x^2 - 15 x +$~\underline{\hspace{.5in}}\\
  7)~ $y^2 - y +$~\underline{\hspace{.5in}}\\
  2)~ $a^2 - 24 a +$~\underline{\hspace{.5in}}\\
  4)~ $x^2 - 34 x +$~\underline{\hspace{.5in}}\\
  6)~ $r^2 - \frac{1}{9} r +$~\underline{\hspace{.5in}}\\
  8)~ $p^2 - 17 p +$~\underline{\hspace{.5in}}
\end{multicols}

{\tmstrong{Solve each equation by completing the square.}}

\begin{multicols}{2}
  9)~ $x^2 - 16 x + 55 = 0$\\
  11)~ $v^2 - 8 v + 45 = 0$\\
  13)~ $6 x^2 + 12 x + 63 = 0$\\
  15)~ $5 k^2 - 10 k + 48 = 0$\\
  17)~ $x^2 + 10 x - 57 = 4$\\
  19)~ $n^2 - 16 n + 67 = 4$\\
  21)~ $2 x^2 + 4 x + 38 = - 6$\\
  23)~ $8 b^2 + 16 b - 37 = 5$\\
  25)~ $x^2 = - 10 x - 29$\\
  27)~ $n^2 = - 21 + 10 n$\\
  29)~ $3 k^2 + 9 = 6 k$\\
  31)~ $2 x^2 + 63 = 8 x$\\
  33)~ $p^2 - 8 p = - 55$\\
  35)~ $7 n^2 - n + 7 = 7 n + 6 n^2$\\
  37)~ $13 b^2 + 15 b + 44 = - 5 + 7 b^2 + 3 b$\\
  39)~ $5 x^2 + 5 x = - 31 - 5 x$\\
  41)~ $v^2 + 5 v + 28 = 0$\\
  43)~ $7 x^2 - 6 x + 40 = 0$\\
  45)~ $k^2 - 7 k + 50 = 3$\\
  47)~ $5 x^2 + 8 x - 40 = 8$\\
  49)~ $m^2 = - 15 + 9 m$\\
  51)~ $8 r^2 + 10 r = - 55$\\
  53)~ $5 n^2 - 8 n + 60 = - 3 n + 6 + 4 n^2$\\
  55)~ $- 2 x^2 + 3 x - 5 = - 4 x^2$\\
~\\
  10)~ $n^2 - 8 n - 12 = 0$\\
  12)~ $b^2 + 2 b + 43 = 0$\\
  14)~ $3 x^2 - 6 x + 47 = 0$\\
  16)~ $8 a^2 + 16 a - 1 = 0$\\
  18)~ $p^2 - 16 p - 52 = 0$\\
  20)~ $m^2 - 8 m - 3 = 6$\\
  22)~ $6 r^2 + 12 r - 24 = - 6$\\
  24)~ $6 n^2 - 12 n - 14 = 4$\\
  26)~ $v^2 = 14 v + 36$\\
  28)~ $a^2 - 56 = - 10 a$\\
  30)~ $5 x^2 = - 26 + 10 x$\\
  32)~ $5 n^2 = - 10 n + 15$\\
  34)~ $x^2 + 8 x + 15 = 8$\\
  36)~ $n^2 + 4 n = 12$\\
  38)~ $- 3 r^2 + 12 r + 49 = - 6 r^2$\\
  40)~ $8 n^2 + 16 n = 64$\\
  42)~ $b^2 + 7 b - 33 = 0$\\
  44)~ $4 x^2 + 4 x + 25 = 0$\\
  46)~ $a^2 - 5 a + 25 = 3$\\
  48)~ $2 p^2 - p + 56 = - 8$\\
  50)~ $n^2 - n = - 41$\\
  52)~ $3 x^2 - 11 x = - 18$\\
  54)~ $4 b^2 - 15 b + 56 = 3 b^2$\\
  56)~ $10 v^2 - 15 v = 27 + 4 v^2 - 6 v$\\
\end{multicols}

\newpage

\subsection{The Quadratic Formula and the Discriminant}

{\tmstrong{Use the discriminant in order to determine the number of real roots for each equation.  If an equation is shown to have one (or two) real root(s), set $y=0$ and use the quadratic formula to find them.}}
\label{QF}
\begin{multicols}{2}
  1)~$y=x^2+2x-1 $\\
  3)~$y=3x^2+12x-1$\\
  5)~$y=x^2+6$\\
  7)~$y=x^2+8x$\\
  9)~$y=x^2+4x-2$\\
  11)~$y=4x^2+10x$\\
	2)~$y=-3x^2-12x-5 $\\
  4)~$y=x^2+2x$\\
  6)~$y=-5x^2-40x$\\
  8)~$y=x^2$\\
  10)~$y=x^2+16x-2 $
\end{multicols}

{\tmstrong{Solve each equation using the quadratic formula.}}

\begin{multicols}{2}
  12)~ $4 a^2 + 6 = 0$\\
  14)~ $2 x^2 - 8 x - 2 = 0$\\
  16)~ $2 m^2 - 3 = 0$\\
  18)~ $3 r^2 - 2 r - 1 = 0$\\
  20)~ $4 n^2 - 36 = 0$\\
  22)~ $v^2 - 4 v - 5 = - 8$\\
  24)~ $2 a^2 + 3 a + 14 = 6$\\
  26)~ $3 k^2 + 3 k - 4 = 7$\\
  28)~ $7 x^2 + 3 x - 16 = - 2$\\
  30)~ $2 p^2 + 6 p - 16 = 4$\\
  32)~ $3 n^2 + 3 n = - 3$\\
  34)~ $2 x^2 = - 7 x + 49$\\
  36)~ $5 x^2 = 7 x + 7$\\
  38)~ $8 n^2 = - 3 n - 8$\\
  40)~ $2 x^2 + 5 x = - 3$\\
  42)~ $4 a^2 - 64 = 0$\\
  44)~ $4 p^2 + 5 p - 36 = 3 p^2$\\
  46)~ $- 5 n^2 - 3 n - 52 = 2 - 7 n^2$\\
  48)~ $7 r^2 - 12 = - 3 r$\\
  50)~ $2 n^2 - 9 = 4$\\
  13)~ $3 k^2 + 2 = 0$\\
  15)~ $6 n^2 - 1 = 0$\\
  17)~ $5 p^2 + 2 p + 6 = 0$\\
  19)~ $2 x^2 - 2 x - 15 = 0$\\
  21)~ $3 b^2 + 6 = 0$\\
  23)~ $2 x^2 + 4 x + 12 = 8$\\
  25)~ $6 n^2 - 3 n + 3 = - 4$\\
  27)~ $4 x^2 - 14 = - 2$\\
  29)~ $4 n^2 + 5 n = 7$\\
  31)~ $m^2 + 4 m - 48 = - 3$\\
  33)~ $3 b^2 - 3 = 8 b$\\
  35)~ $3 r^2 + 4 = - 6 r$\\
  37)~ $6 a^2 = - 5 a + 13$\\
  39)~ $6 v^2 = 4 + 6 v$\\
  41)~ $x^2 = 8$\\
  43)~ $2 k^2 + 6 k - 16 = 2 k$\\
  45)~ $12 x^2 + x + 7 = 5 x^2 + 5 x$\\
  47)~ $7 m^2 - 6 m + 6 = - m$\\
  49)~ $3 x^2 - 3 = x^2$\\
  51)~ $6 b^2 = b^2 + 7 - b$
\end{multicols}

\newpage

%\subsection{Applications}

%\newpage

\subsection{Quadratic Inequalities and Sign Diagrams}

{\tmstrong{Construct a sign diagram for each of the following expressions/equations.  Then using interval notation, describe the set of values for which the given expression is greater than or equal to zero.}}\pp

1) - 5): Expressions (1) through (5) on page \pageref{ais1}.\pp

6) - 10): Expressions (1) through (5) on page \pageref{aisnot1}.\pp

11) - 15): Expressions (21) through (25) on page \pageref{aisnot1}.\pp

16) - 20): Equations (1) through (5) on page \pageref{QF}.\pp
